# baseURI: http://github.com/common-workflow-language
# imports: http://purl.org/wf4ever/wfdesc

@prefix cnt: <http://www.w3.org/2011/content#> .
@prefix cwl: <http://github.com/common-workflow-language#> .
@prefix owl: <http://www.w3.org/2002/07/owl#> .
@prefix rdf: <http://www.w3.org/1999/02/22-rdf-syntax-ns#> .
@prefix rdfs: <http://www.w3.org/2000/01/rdf-schema#> .
@prefix sch: <http://schema.org/> .
@prefix wfdesc: <http://purl.org/wf4ever/wfdesc#> .
@prefix wfprov: <http://purl.org/wf4ever/wfprov#> .
@prefix xsd: <http://www.w3.org/2001/XMLSchema#> .

<http://github.com/common-workflow-language>
  owl:imports <http://purl.org/wf4ever/wfdesc> ;
.
cwl:Adapter
  rdf:type owl:Class ;
  rdfs:comment "Base class for ArgumentAdapter and OutputAdapter."^^xsd:string ;
  rdfs:subClassOf owl:Thing ;
.
cwl:App
  rdf:type owl:Class ;
  rdfs:subClassOf wfdesc:Process ;
  rdfs:subClassOf owl:Thing ;
.
cwl:ArgumentAdapter
  rdf:type owl:Class ;
  rdfs:comment "Describes how to map values known at runtime (or literals) to command line."^^xsd:string ;
  rdfs:subClassOf cwl:Adapter ;
.
cwl:AvroTypeDef
  rdf:type owl:Class ;
  rdfs:comment "Type definition compatible with Apache Avro"^^xsd:string ;
  rdfs:subClassOf cwl:ParameterSchema ;
.
cwl:CommandLineTool
  rdf:type owl:Class ;
  rdfs:comment "Adapts a CLI tool to be runnable in CWL engines and used in workflows."^^xsd:string ;
  rdfs:subClassOf cwl:App ;
.
cwl:ContainerRequirement
  rdf:type owl:Class ;
  rdfs:comment "Signifies that a Process (CommandLineTool) needs to run within a linux container."^^xsd:string ;
  rdfs:subClassOf cwl:Requirement ;
.
cwl:DockerContainer
  rdf:type owl:Class ;
  rdfs:comment "Signifies the process (CommandLineTool) needs to run in a Docker container. Image is specified using cwl:hasImageSpec."^^xsd:string ;
  rdfs:subClassOf cwl:ContainerRequirement ;
.
cwl:File
  rdf:type owl:Class ;
  rdfs:comment "File content specified through cnt:contentUrl in absolute paths. Additional triples that can be propagated to files produced by workflows should be kept in a node referenced through cwl:hasAnnotations. Likewise, for accompanying index files, use cwl:hasIndexFile. TODO: Add file properties and look for a possible base class."^^xsd:string ;
  rdfs:subClassOf owl:Thing ;
.
cwl:IndexFile
  rdf:type owl:Class ;
  rdfs:comment "Index files accompany data files and follow a naming convention."^^xsd:string ;
  rdfs:subClassOf cwl:File ;
.
cwl:LiteralOrTransform
  rdf:type owl:Class ;
  rdfs:subClassOf owl:Thing ;
.
cwl:OutputAdapter
  rdf:type owl:Class ;
  rdfs:comment "Describes how to report process outputs from generated files. This includes file metadata and accompanying index files."^^xsd:string ;
  rdfs:subClassOf cwl:Adapter ;
.
cwl:ParameterSchema
  rdf:type owl:Class ;
  rdfs:comment "TODO: subclass with AvroTypeDefinition"^^xsd:string ;
  rdfs:subClassOf owl:Thing ;
.
cwl:RequiredCPU
  rdf:type owl:Class ;
  rdfs:subClassOf cwl:ResourceRequirement ;
.
cwl:RequiredMemory
  rdf:type owl:Class ;
  rdfs:subClassOf cwl:ResourceRequirement ;
.
cwl:Requirement
  rdf:type owl:Class ;
  rdfs:comment "Base class for requirements a Process needs to run."^^xsd:string ;
  rdfs:subClassOf owl:Thing ;
.
cwl:ResourceRequirement
  rdf:type owl:Class ;
  rdfs:comment "Describes what computational resources a process needs to run (#CPU, RAM). Used for CommandLineTools. Actual value supplied via rdf:value which can point to cwl:Transformation for dynamic requirements."^^xsd:string ;
  rdfs:subClassOf cwl:Requirement ;
.
cwl:Transform
  rdf:type owl:Class ;
  rdfs:comment "Transformation that can be applied to values known at runtime. Specify via rdf:value and cwl:hasLanguage"^^xsd:string ;
  rdfs:subClassOf cwl:LiteralOrTransform ;
.
cwl:WorkflowEngineFeature
  rdf:type owl:Class ;
  rdfs:comment "Class for CWL extension features."^^xsd:string ;
  rdfs:subClassOf cwl:Requirement ;
.
cwl:argumentValue
  rdf:type owl:ObjectProperty ;
  rdfs:comment "Defines how to get the value at runtime in order to map it to command line argument. Target is usually a cwl:Transformation but can be a literal."^^xsd:string ;
  rdfs:domain cwl:ArgumentAdapter ;
  rdfs:range cwl:LiteralOrTransform ;
.
cwl:avroDoc
  rdf:type owl:DatatypeProperty ;
  rdfs:comment "Describes Avro schema definition. Used for UI generation. TODO: subproperty of rdfs:comment?"^^xsd:string ;
  rdfs:domain cwl:AvroTypeDef ;
  rdfs:range xsd:string ;
.
cwl:avroFields
  rdf:type owl:ObjectProperty ;
  rdfs:domain cwl:AvroTypeDef ;
  rdfs:range rdf:List ;
.
cwl:avroItemType
  rdf:type owl:DatatypeProperty ;
  rdfs:comment "Specifies one or more item types for Avro array type."^^xsd:string ;
  rdfs:domain cwl:AvroTypeDef ;
  rdfs:range xsd:string ;
.
cwl:avroName
  rdf:type owl:DatatypeProperty ;
  rdfs:comment "Specifies Avro type name. It needs to be unique within the process description and cannot be \"File\"."^^xsd:string ;
  rdfs:domain cwl:AvroTypeDef ;
  rdfs:range xsd:string ;
.
cwl:avroSymbols
  rdf:type owl:ObjectProperty ;
  rdfs:domain cwl:AvroTypeDef ;
  rdfs:range rdf:List ;
.
cwl:avroType
  rdf:type owl:DatatypeProperty ;
  rdfs:domain cwl:AvroTypeDef ;
  rdfs:label "Specifies Avro type. TODO: range enum"^^xsd:string ;
  rdfs:range xsd:string ;
.
cwl:hasAdapter
  rdf:type owl:ObjectProperty ;
  rdfs:comment "A way to embed adapters with schema."^^xsd:string ;
  rdfs:domain cwl:AvroTypeDef ;
  rdfs:range cwl:Adapter ;
.
cwl:hasArgumentAdapters
  rdf:type owl:ObjectProperty ;
  rdfs:comment "Specifies additional adapters for CommandLineTool. Elements are cwl:ArgumentAdapter"^^xsd:string ;
  rdfs:domain cwl:CommandLineTool ;
  rdfs:range rdf:List ;
.
cwl:hasBaseArguments
  rdf:type owl:ObjectProperty ;
  rdfs:comment "A list of used as base for building command line arguments. If any element is cwl:Transformation, it will be applied at runtime."^^xsd:string ;
  rdfs:domain cwl:CommandLineTool ;
  rdfs:range rdf:List ;
.
cwl:hasCommandLinePosition
  rdf:type owl:DatatypeProperty ;
  rdfs:comment "Used to order values when building command line arguments. Lower takes priority."^^xsd:string ;
  rdfs:domain cwl:ArgumentAdapter ;
  rdfs:range xsd:integer ;
.
cwl:hasDepth
  rdf:type owl:DatatypeProperty ;
  rdfs:comment "Specifies nesting depth of inputs and outputs. Zero for no nesting. If unspecified, depth is considered to be \"any\"."^^xsd:string ;
  rdfs:domain wfdesc:Parameter ;
  rdfs:range xsd:nonNegativeInteger ;
.
cwl:hasDockerImageId
  rdf:type owl:DatatypeProperty ;
  rdfs:comment "Specifies ID of docker image. ID is also the checksum."^^xsd:string ;
  rdfs:domain cwl:DockerContainer ;
  rdfs:range xsd:string ;
.
cwl:hasDockerRepository
  rdf:type owl:DatatypeProperty ;
  rdfs:comment "Specifies docker repository. For repos on main docker index, this is the name optionally prefixed with namespace. For other repositories, this is the URL."^^xsd:string ;
  rdfs:domain cwl:DockerContainer ;
  rdfs:range xsd:string ;
.
cwl:hasDockerRepositoryTag
  rdf:type owl:DatatypeProperty ;
  rdfs:comment "Specifies docker repository tag without leading \"#\"."^^xsd:string ;
  rdfs:domain cwl:DockerContainer ;
  rdfs:range xsd:string ;
.
cwl:hasGlob
  rdf:type owl:ObjectProperty ;
  rdfs:comment "Output adapters select produced files using a glob expression. Range is either string or Transform."^^xsd:string ;
  rdfs:domain cwl:OutputAdapter ;
  rdfs:range cwl:LiteralOrTransform ;
.
cwl:hasIndexFile
  rdf:type owl:ObjectProperty ;
  rdfs:comment "Files have accompanying index files based on a naming convention."^^xsd:string ;
  rdfs:domain cwl:File ;
  rdfs:range cwl:IndexFile ;
.
cwl:hasItemSeparator
  rdf:type owl:DatatypeProperty ;
  rdfs:comment "Used for mapping lists to command line."^^xsd:string ;
  rdfs:domain cwl:ArgumentAdapter ;
  rdfs:range xsd:string ;
.
cwl:hasLanguage
  rdf:type owl:DatatypeProperty ;
  rdfs:comment "Programing language of subject Transformation. TODO: Consider making it object property and using dbpedia for vocab."^^xsd:string ;
  rdfs:domain cwl:Transform ;
  rdfs:range xsd:string ;
.
cwl:hasPrefix
  rdf:type owl:DatatypeProperty ;
  rdfs:comment "Used for building command line arguments."^^xsd:string ;
  rdfs:domain cwl:ArgumentAdapter ;
  rdfs:range xsd:string ;
.
cwl:hasRequirement
  rdf:type owl:ObjectProperty ;
  rdfs:comment "Associates a Process with its requirements to run. Multiple cwl:hasRequirements are to be interpreted as oneOf, not allOf."^^xsd:string ;
  rdfs:domain cwl:App ;
  rdfs:range cwl:Requirement ;
.
cwl:hasSchema
  rdf:type owl:ObjectProperty ;
  rdfs:comment "Associates a Parameter with its schema. It should only have one."^^xsd:string ;
  rdfs:domain wfdesc:Parameter ;
  rdfs:range cwl:AvroTypeDef ;
.
cwl:hasSeparator
  rdf:type owl:DatatypeProperty ;
  rdfs:comment "Used for building command line arguments."^^xsd:string ;
  rdfs:domain cwl:ArgumentAdapter ;
  rdfs:range xsd:string ;
.
cwl:hasStdin
  rdf:type owl:ObjectProperty ;
  rdfs:comment "Value produced by object of this property is a file path for stdin. TODO: range should be string or transformation"^^xsd:string ;
  rdfs:domain cwl:CommandLineTool ;
  rdfs:range cwl:LiteralOrTransform ;
.
cwl:hasStdout
  rdf:type owl:ObjectProperty ;
  rdfs:comment "Value produced by object of this property is a file path for stdout. TODO: range should be string or transformation"^^xsd:string ;
  rdfs:domain cwl:CommandLineTool ;
  rdfs:range cwl:LiteralOrTransform ;
.
cwl:includeIndexFile
  rdf:type owl:DatatypeProperty ;
  rdfs:domain cwl:OutputAdapter ;
  rdfs:range xsd:string ;
.
cwl:isStreamable
  rdf:type owl:DatatypeProperty ;
  rdfs:comment "Signifies that files on associated input or output can be streamed (the tool does not perform seeks)."^^xsd:string ;
  rdfs:domain cwl:Adapter ;
  rdfs:range xsd:boolean ;
.
cwl:modifiesMountedDirectory
  rdf:type owl:DatatypeProperty ;
  rdfs:comment "Signifies that the tool will modify the directories where files from this input are located."^^xsd:string ;
  rdfs:domain cwl:ArgumentAdapter ;
  rdfs:range xsd:boolean ;
.
cwl:usesSchema
  rdf:type owl:ObjectProperty ;
  rdfs:comment "Used for parameters with complex structures. Process can define schema classes using this property and they will be available for reference in parameter schema definitions."^^xsd:string ;
  rdfs:domain cwl:App ;
  rdfs:range cwl:AvroTypeDef ;
.
<http://rabix.org/cwl>
  rdf:type owl:Ontology ;
  owl:imports <http://purl.org/wf4ever/wfdesc> ;
  owl:imports <http://purl.org/wf4ever/wfprov> ;
.
